Modify open to raise exn when given bad filename
This requires the ffi model to signal the error condition in the
returned byte array rather than simply cause an FFI failure, as it was
doing previously.

compiler/bootstrap/io/catfileSystemScript.sml
@@ -10,6 +10,7 @@ val _ = overload_on ("SOME", ``SOME``)
 val _ = overload_on ("NONE", ``NONE``)
 val _ = overload_on ("monad_bind", ``OPTION_BIND``)
 val _ = overload_on ("monad_unit_bind", ``OPTION_IGNORE_BIND``)
+val _ = overload_on ("++", ``OPTION_CHOICE``)
 
 (* TODO: move candidates follow *)
 val ALOOKUP_EXISTS_IFF = Q.store_thm(
@@ -364,9 +365,9 @@ val fs_ffi_next_def = Define`
       | 1 => do (* open file *)
                fname <- getNullTermStr bytes;
                (fd, fs') <- openFile fname fs;
-               assert(fd < 256);
+               assert(fd < 255);
                return (LUPDATE (n2w fd) 0 bytes, encode fs')
-             od
+             od ++ return (LUPDATE 255w 0 bytes, encode fs)
       | 2 => do
                assert(LENGTH bytes = 1);
                (copt, fs') <- fgetc (w2n (HD bytes)) fs;
